ajout de plein de fichiers

examples/Sek/Owner.ml
@@ -1,0 +1,4 @@
+type owner = unit ref
+
+let none = ref ()
+let fresh_id () = ref ()
