examples/Sek/PArray.ml
@@ -1,6 +1,6 @@
 (** Persistent arrays. *)
 type 'a parray = {
-  mutable data : 'a parray_desc;
+  mutable desc : 'a parray_desc;
   mutable maxdist : int } (* TODO: maxdist *)
 
 and 'a parray_desc =
@@ -13,7 +13,7 @@ let dist_bound a =
 (* TODO
 
 let mk_base a =
-  { data = PArray_Base a;
+  { desc = PArray_Base a;
     maxdist = 0 }
 
 *)
@@ -22,12 +22,12 @@ let mk_base a =
   creates a fresh persistent array of size [sz] filled with default value [d]. *)
 let parray_create sz d =
   let a = Array.make sz d in
-  { data = PArray_Base a;
+  { desc = PArray_Base a;
     maxdist = 0 }
 
 (* On coupe la chaîne avec un nouveau tableau contenant toutes les modifications de la version. *)
 let rec parray_base_copy pa =
-  match pa.data with
+  match pa.desc with
   | PArray_Base a -> Array.copy a
   | PArray_Diff (origin, index, value) ->
     let a = parray_base_copy origin in
@@ -35,11 +35,11 @@ let rec parray_base_copy pa =
     a
 
 let parray_rebase_and_get_array pa =
-  match pa.data with
+  match pa.desc with
   | PArray_Base a -> a
   | PArray_Diff (origin, _, _) ->
     let a = parray_base_copy pa in
-    pa.data <- PArray_Base a;
+    pa.desc <- PArray_Base a;
     a
 
 let parray_get pa i =
@@ -52,26 +52,26 @@ let parray_set pa i x =
   if cond then begin
     let b = Array.copy a in
     b.(i) <- x;
-    { data = PArray_Base b;
+    { desc = PArray_Base b;
       maxdist = 0 }
   end else begin
     let v = a.(i) in
     a.(i) <- x;
     let pb = {
-      data = PArray_Base a;
+      desc = PArray_Base a;
       maxdist = pa.maxdist + 1 } in
-    pa.data <- PArray_Diff (pb, i, v);
+    pa.desc <- PArray_Diff (pb, i, v);
     pb
   end
 
 let parray_copy pa =
   let a = parray_base_copy pa in
-  { data = PArray_Base a;
+  { desc = PArray_Base a;
     maxdist = 0 }
 
 (** [parray_of_array a]
   returns a persistent version of [a].
   This function is destructive and [a] may not be used again after calling it. *)
 let parray_of_array a =
-  { data = PArray_Base a;
+  { desc = PArray_Base a;
     maxdist = 0 }
